\documentclass[letterpaper, 10pt]{article}
% --- Input encoding ---
\usepackage{ucs}
\usepackage[utf8x]{inputenc}
\usepackage[english]{babel}
% --- Fonts ---
\usepackage[T1]{fontenc}
\usepackage{lmodern}
\usepackage{textcomp}
%\usepackage{times}
%\usepackage{ae,aecompl}
% --- Graphics ---
\usepackage{tikz}
\usepackage{pgf}
\usepackage{pgfplots}
\usepackage{pgffor}
\usepgflibrary{plothandlers}
\pgfplotsset{plot coordinates/math parser=true}
\pgfplotsset{compat=newest}
\usetikzlibrary{plotmarks}
\usepackage{graphicx}
\usepackage{epsfig}

\usepackage{amsmath, amssymb, graphics, setspace, units, fancyvrb, hyperref}

\newcommand{\mathsym}[1]{{}}
\newcommand{\unicode}[1]{{}}


\begin{document}
	
	\section*{Task 1a} % (fold)
	\label{sec:Task 1a}
	As salt can not penetrate the interface: $\dot{m}_s'' = Y_s \dot{m}'' + j_s = 0$ and $j_s = -\rho_l D \frac{\partial Y_s}{\partial y}\big|_{y=0}$ where $Y_s = \frac{s}{1000}$ is the mass fraction of salt present and at the interface $Y_s = \frac{s_0}{1000}$.\\
		
	\noindent $Y_s \dot{m}'' = \rho_l D \frac{\partial Y_s}{\partial y}\big|_{y=0}$\\
	\noindent $\dot{m}'' = \rho_l V_l + \rho_s V_s$ where $V_l = V_0$ and $V_s = 0$ as salt has no velocity.\\
	
	\noindent $Y_s \rho_l V_0 = \rho_l D \frac{\partial Y_s}{\partial y}\big|_{y=0}$\\
	
	\noindent where $V_0 = \frac{k}{\left(1-\frac{s_0}{1000}\right)\rho_l \hat{h_{il}}} \frac{\partial T}{\partial y}\big|_{y=0}$\\
	
	\noindent $Y_s  \frac{k}{\left(1-\frac{s_0}{1000}\right)\rho_l \hat{h_{il}}} \frac{\partial T}{\partial y}\big|_{y=0} = D  \frac{\partial Y_s}{\partial y}\big|_{y=0}$\\
	
	\noindent $\frac{s_0}{1000} \cdot \frac{k}{\left(1-\frac{s_0}{1000}\right)\rho_l \hat{h_{il}}} \frac{\partial T}{\partial y}\big|_{y=0} = D  \frac{\partial \frac{s_0}{1000} }{\partial y}\big|_{y=0}$\\
	
	\noindent $1000 \frac{k}{\hat{h_{il}}} \frac{\partial T}{\partial y}\big|_{y=0} = \left(\frac{1000-s_0}{s_0}\right) \rho_l D \frac{\partial s_0}{\partial y}\big|_{y=0} $\\
	
	Thus, $C_1 = 1000 $\\
	
	% section Task 1a (end)
	
	\section*{Task 1b} % (fold)
	\label{sec:Task 1b}

	\begin{align*}
		\rho_m[s]&:=\rho_{m0}(1+g_1 s)\\
		\alpha[s]&:=\alpha_0(1+g_2 s)\\
		T_m[s]&:=T_{m0}*(1+g_3 s)\\
		\rho[T,s]&:=\rho_m[s]*\left(1-\alpha[s] |T-T_m[s]|^q\right)\\
		\rho_l&:=\rho_m[s_\infty]\\
		\phi&:=\frac{T-T_\infty}{T_0-T_\infty}\\
		S&:=\frac{s-s_\infty}{s_0-s_\infty}\\
		R&:=\frac{T_m[s_\infty]-T_\infty}{T_0-T_\infty}\\
		A&:=\frac{g_1*\rho_{m0}*(s_0-s_\infty)}{\rho_m[s_\infty]}\\
		B&:=\frac{g_2*\alpha_0*(s_0-s_\infty)}{\alpha[s_\infty]}\\
		Q&:=\frac{g_3*T_{m0}*(s_0-s_\infty)}{T_0-T_\infty}\\
		P&:=\frac{g_1*\rho_{m0}(s_0-s_\infty)}{\rho_m[s_\infty]*\alpha[s_\infty]*|T_0-T_\infty|^q}\\
	\end{align*}

	Plugging all of these equations into the right and left hand sides of the relation to be proves is as follows:

	\begin{multline*}
		RHS\\
		= \rho_m[s_\infty] \alpha[s_\infty] |T_0-T_\infty|^q \left((1+A*S)*(1+B*S)*|\phi 	-R-Q*S|^q-|R|^q-P*S\right) \\
		= (1+g_1 s_\infty) (1+g_2 s_\infty) \alpha_0 \rho_{m0} |T_0-T_\infty|^q \cdot \\
		\left(\frac{\left(g_1 (-s+s_\infty)+(1+g_1 s) (1+g_2 s) \alpha_0 |-T+T_{m0}+g_3 s T_{m0}|^q\right)
		|T_0-T_\infty|^{-q}}{(1+g_1 s_\infty) (1+g_2 s_\infty) \alpha_0}\right) -\\ 
		\shoveleft{\left|\frac{T_{m0}+g_3 s_\infty T_{m0}-T_\infty}{T_0-T_\infty}\right|^q}
	\end{multline*}

	\begin{multline*}
		LHS\\
		= \rho[T_\infty,s_\infty]-\rho [T,s]\\ 
		= \rho_{m0} (g_1 (-s+s_\infty)+(1+g_1 s) \cdot \\
		(1+g_2 s) \alpha_0 |T-(1+g_3 s) T_{m0}|^q-(1+g_1 s_\infty) \cdot\\ 
		(1+g_2 s_\infty) \alpha_0 |T_{m0}+g_3 s_\infty T_{m0}-T_\infty|^q)
	\end{multline*}

	Comparing the RHS to the LHS of of the equation and simplifying we are thus able to show their equivalence.
	% section Task 1b (end)

	\section*{Task 1c} % (fold)
	\label{sec:Task 1b}
	With the definitions of Temperature and Salinity in terms of S and $\phi$:\\
	T := $T_\infty$ + $\phi$*($T_0$-$T_\infty$)\\
	s := $s_\infty $ + S* ($s_0$ - $s_\infty $)\\
	$Gr_x$ := CGr * $x^3$ for CGr := $\frac{\rho_{m0}}{\rho_m (s_\infty)}\frac{g g_1 (s_\infty-s_0)}{(\mu/\rho_l)^2}$\\

	\noindent Employing the similiarty transformation as given:\\ 
	$\eta$ = $\frac{y}{\sqrt{2}x} Gr_x^{1/4}$ and $\psi$ = $\frac{4}{\sqrt{2}}\frac{\mu}{\rho_l} Gr_x^{1/4} f(\eta)$\\

	\noindent Velocities can be found as:\\
	u := $\partial_\eta \psi [x,\eta ]*\partial _y\eta [x,y]$ = $\frac{2 \mu  \sqrt{Gr_x} f'(\eta )}{\rho_l x}$\\
	v := $-\left(\partial _x\psi [x,\eta ]+\partial _{\eta }\psi [x,\eta ]*\partial _x\eta [x,y]\right) $ = \\ - $\frac{2 \sqrt{2} \mu  \sqrt[4]{Gr_x} \left(\frac{3 \text{CGr} x y}{4 \sqrt{2} \left(Gr_x\right)^{3/4}}-\frac{y \sqrt[4]{Gr_x}}{\sqrt{2} x^2}\right) f'(\eta )}{\rho_l}-\frac{3 \text{CGr} \mu  x^2 f(\eta )}{\sqrt{2} \rho_l \left(Gr_x\right)^{3/4}}$

	\noindent The advective derivatives simiarly follow as:\\ 
	$\frac{\partial u}{\partial y}$ = $\partial _{\eta ,\eta }\psi [x,\eta ]*\left(\partial _y\eta [x,y]\right){}^2$ = $\frac{\sqrt{2} \mu  \left(Gr_x\right)^{3/4} f''(\eta )}{\rho_l x^2}$\\
	$\frac{\partial u}{\partial x}$ = $\partial _{\eta }\psi [x,\eta ]*\partial _{x,y}\eta [x,y]+\partial _{x,\eta }\psi [x,\eta ]*\partial _y\eta [x,y]+\partial
	_{\eta ,\eta }\psi [x,\eta ]*\partial _x\eta [x,y]*\partial _y\eta [x,y]$ =  $\frac{2 \mu  \sqrt{Gr_x} \left(\frac{3 \text{CGr} x y}{4 \sqrt{2} \left(Gr_x\right)^{3/4}}-\frac{y \sqrt[4]{Gr_x}}{\sqrt{2} x^2}\right) f''(\eta )}{\rho_l x}+\frac{3 \text{CGr} \mu  x f'(\eta )}{2 \rho_l \sqrt{Gr_x}}+\frac{2 \sqrt{2}\mu  \sqrt[4]{Gr_x} \left(\frac{3 \text{CGr} x}{4 \sqrt{2} \left(Gr_x\right)^{3/4}}-\frac{\sqrt[4]{Gr_x}}{\sqrt{2} x^2}\right) f'(\eta )}{\rho_l}$ \\

	\noindent The laplacian term is now given as:\\
	$\frac{\partial^2 u}{\partial y^2}$ = $\partial _{\eta ,\eta ,\eta }\psi [x,\eta ]*\left(\partial _y\eta [x,y]\right){}^3$ = $\frac{\text{CGr} \mu  f^{(3)}(\eta )}{\rho_l}$\\

	\noindent The corresponding derivatives for the energy equation are:\\
	$\frac{\partial T}{\partial x}$ = $\partial _{\phi }T*\phi '*\partial _x\eta [x,y]$ = 
	$(T_0-T_\infty) \phi ' \left(\frac{3 \text{CGr} x y}{4 \sqrt{2} \left(Gr_x\right)^{3/4}}-\frac{y \sqrt[4]{Gr_x}}{\sqrt{2} x^2}\right)$\\
	$\frac{\partial T}{\partial y}$ = $ \partial _{\phi }T*\phi '*\partial _y\eta [x,y]$ = $\frac{\sqrt[4]{Gr_x} (T_0-T_\infty) \phi '}{\sqrt{2} x}$\\
	$\frac{\partial^2 T}{\partial y^2}$ = $\partial _{\phi }T*\phi \text{''}*\left(\partial _y\eta [x,y]\right){}^2$ = $\frac{\sqrt{Gr_x} (T_0-T_\infty) \phi ''}{2 x^2}$\\

	\noindent The derivatives for the species equation are:\\
	$\frac{\partial s}{\partial x}$ = $\partial _Ss * S'*\partial _x\eta [x,y]$ = $S' (s_0-s_\infty) \left(\frac{3 \text{CGr} x y}{4 \sqrt{2} \left(Gr_x\right)^{3/4}}-\frac{y \sqrt[4]{Gr_x}}{\sqrt{2} x^2}\right)$\\
	$\frac{\partial s}{\partial y}$ = $\partial _Ss * S'*\partial _y\eta [x,y]$ = $\frac{\sqrt[4]{Gr_x} S' (s_0-s_\infty)}{\sqrt{2} x}$\\
	$\frac{\partial^2 s}{\partial y^2}$ = $\partial _Ss* S\text{''}*\left(\partial _y\eta [x,y]\right){}^2$ = $\frac{\sqrt{Gr_x} S'' (s_0-s_\infty)}{2 x^2}$\\

	\noindent Putting together the momentum equation:\\
	$u*\frac{\partial u}{\partial x}+v*\frac{\partial u}{\partial y}-\frac{g(\rho_\infty -\rho )}{\rho_l}-\left(\frac{\mu }{\rho_l}\right)\frac{\partial^2 u}{\partial y^2} = 0$\\

	\noindent Dividing by $\left(\frac{Gr_x\mu ^2}{ \rho_l^2 x^3}\right)$ and factoring yeilds:\\
	$-\frac{4 Gr_x f'(\eta )^2}{Gr_x}+\frac{g \rho  \rho_l}{\text{CGr} \mu^2}-\frac{g \rho_l \rho_\infty}{\text{CGr} \mu^2}-f^{(3)}(\eta )-3 f(\eta ) f''(\eta )+6 f'(\eta )^2 = 0$\\

	\noindent Simplifying and canceling terms, we arrive at:\\
	$f^{(3)}(\eta )-3 f(\eta ) f''(\eta )+2 f'(\eta )^2 + \frac{g (\rho_\infty - \rho) \rho_l}{\text{CGr} \mu^2} = 0 $\\

	\noindent Also, the final term on the right hand side can be written as:\\ 
	$\frac{g (\rho_\infty - \rho) \rho_l}{\text{CGr} \mu^2}$ = $\frac{(\rho_\infty - \rho)}{g_1 \rho_{m0} (s_\infty - s_0)}$\\ 
 
	\noindent Where: $P := \frac{g_1 \rho_{m0} (s_\infty - s_0)}{\rho_m (s_\infty) \alpha (s_\infty) |T_0 - T_\infty|^2}$\\ 
	and $W := -\frac{1}{P}\left[ (1+AS)(1+BS)|1-R-QS|^q-|R|^q-PS\right]$\\

	Thus, finally yeilding:\\
	\begin{center}
		$f^{(3)}(\eta )-3 f(\eta ) f''(\eta )+2 f'(\eta )^2 + W = 0 $ for $C_2 = 1$
	\end{center}

	\noindent For the energy equation:\\
	$u*\frac{\partial t}{\partial x}+v*\frac{\partial t}{\partial y}-\frac{k}{\rho_l*\text{cp}}*\frac{\partial^2 t}{\partial y^2} = 0$\\

	\noindent Dividing through by $\left(-\frac{k \sqrt{Gr_x} (T_0-T_\infty)}{2 \text{cp} \rho_l x^2}\right)$ and simplifying:\\
	\begin{center}
		$\frac{3 \text{cp} \mu  f(\eta ) \phi'}{k}+\phi'' = 0$ where $Pr := \frac{\text{cp} \mu}{k}$\\
	\end{center}
	For the species equation:\\
	$u*\frac{\partial s}{\partial x}+v*\frac{\partial s}{\partial y}-D*\frac{\partial^2 s}{\partial y^2} = 0$\\

	\noindent Dividing through by $\frac{D(s_0-s_\infty)\sqrt{Gr_x}}{2 x^2}$ and simplifying yeilds:\\
	\begin{center}
		$-\frac{3 \mu  f(\eta ) S'}{D \rho_l}-S'' = 0$ where $Sc := \frac{\mu}{D \rho_l} $
	\end{center}

	% section Task 1c (end)

	\section*{Task 1c boundary condition proof} % (fold)
	\label{sec:Task 1c}
	Begining with the equation: $\left( \frac{1000-s_0}{s_0} \right) D \rho_l \left( \frac{\partial s}{\partial y} \right)_{y = 0}$ = $1000 \frac{k}{\hat{h_{il}}}  \left (\frac{\partial T}{\partial y} \right)_{y = 0}$\\

	\noindent And the non-dimentional definitions for salinity and temperature as follows:\\
	\begin{center}
		$\phi = \frac{T-T_\infty}{T_0-T_\infty}$ and $S = \frac{s - s_\infty}{s_0 - s_\infty}$
	\end{center}

	\noindent rearranging yeilds:\\
	\begin{center}
		T := $T_\infty$ + $\phi$*($T_0$-$T_\infty$) and s := $s_\infty $ + S* ($s_0$ - $s_\infty $)
	\end{center}

	\noindent Derivatives follow as:\\
	\begin{align*}
		\frac{\partial s}{\partial y} &= \frac{\partial S}{\partial y}(s_0 - s_\infty) & 		\frac{\partial T}{\partial y} &= \frac{\partial \phi}{\partial y}(T_0 - T_\infty)\\
		\frac{\partial S}{\partial y} &=  \frac{\partial S}{\partial \eta}  \frac{\partial \eta}{\partial y} & \frac{\partial \phi}{\partial y} &=  \frac{\partial \phi}{\partial \eta}\frac{\partial \eta}{\partial y}\\
	\end{align*}

	\noindent Plugging those definitions into the original equation:\\
	$\left(\frac{1000 - s_0}{s_0}\right) \rho_l D (s_0 - s_\infty) \left(\frac{\partial S}{\partial \eta}\right)_{\eta = 0} \frac{\partial \eta}{\partial y} = 1000 \frac{k}{\hat{h_{il}}} (T_0 - T_\infty) \left(\frac{\partial \phi}{\partial \eta}\right)_{\eta = 0}\frac{\partial \eta}{\partial y}$\\

	\noindent If we define $S' = \frac{\partial S}{\partial \eta} $ and $ \phi ' = \frac{\partial \phi}{\partial \eta}$, we can rearrange the origninal equation as follows:\\

	$\frac{S'(0)}{\phi'(0)} = \frac{1000 k (T_0 - T_\infty)}{\hat{h_{il}} \rho_l D (s_0 - s_\infty)\left(\frac{1000 - s_0}{s_0}\right)}$\\

	\noindent and for $Pr = \frac{\nu}{\alpha} = \frac{c_p \mu}{k}$ and $Sc = \frac{\nu}{D}=\frac{\mu}{\rho D}$, then $\frac{k}{\rho_l D} = \frac{Sc}{Pr}c_p$\\

	We finally arrive at:\\
	\begin{center}
		$\frac{S'(0)}{\phi'(0)} = \frac{Sc}{Pr}\frac{s_0 c_p (T_0 - T_\infty)}{\hat{h_{il}} (s_0 - s_\infty) \left(\frac{1000 - s_0}{s_0} \right) }$
	\end{center}

 

	% section Task 1c (end)

\end{document}
