\section*{Task 2} % (fold)
\label{sec:Task 2}
	\subsection*{Task 2a}
	We are now to change the coordinates from $\eta$ to $\zeta$ using the following transformation
	\begin{align*}
	  F(\zeta) =& (3\text{Pr})^{3/4} f(\eta) & \zeta =& (3 \text{Pr})^{1/4} \\
	  \bar{\phi}(\zeta) =& \phi (\eta) & \bar{S}(\zeta) =& S(\eta )\\
	\end{align*}

	we can begin by applying the chain rule to the derivatives. Since $\zeta$ is a linear function of $\eta$ all terms including higher derivatives than the first one drop out.
	\begin{align*}
	  \frac{\partial^3 f}{\partial \eta^3}=& \left( \frac{\partial \zeta}{\partial \eta} \right)^3 \frac{\partial^3 f}{\partial \zeta^3}=(3 \text{Pr})^{3/4}f'''=F'''\\
	  \frac{\partial^2 f}{\partial \eta^2}=& \left( \frac{\partial \zeta}{\partial \eta} \right)^2 \frac{\partial^2 f}{\partial \zeta^2}=(3 \text{Pr})^{1/2}f''=(3 \text{Pr})^{-1/4} F''\\
	  \frac{\partial f}{\partial \eta}=& \left( \frac{\partial \zeta}{\partial \eta} \right) \frac{\partial f}{\partial \zeta}=(3 \text{Pr})^{1/4}f'=(3 \text{Pr})^{-1/2}F'
	\end{align*}
	Inserting those relations into the momentum equation gives
	\begin{align*}
	  &f'''+3f\cdot f'' -2(f')^2 + 1 \bar{W} = 0 \\
	  \Rightarrow& F''' +\frac{1}{\text{Pr}}F\cdot F'' -\frac{2}{3}\frac{1}{\text{Pr}}+\bar{W}=0 
	\end{align*}
	revealing $C_3$ = 1, and when the Prandtl number approaches infinity this gives
	\begin{equation*}
	  \lim_{\text{Pr}\rightarrow \infty} (\text{Mom}) = F'''+\bar{W} =0
	\end{equation*}

	This can similarly be done for the energy equation
	\begin{align*}
	  \frac{\partial^2 \phi}{\partial \eta^2}=& \left( \frac{\partial \zeta}{\partial \eta} \right)^2 \frac{\partial^2 \phi}{\partial \zeta^2}=(3 \text{Pr})^{1/2}\phi'' =(3 \text{Pr})^{1/2}\bar{\phi}'' \\
	  \frac{\partial \phi}{\partial \eta}=& \left( \frac{\partial \zeta}{\partial \eta} \right) \frac{\partial \phi}{\partial \zeta}=(3 \text{Pr})^{1/4}\phi' =(3 \text{Pr})^{1/4}\bar{\phi}' 
	\end{align*}
	Applying this to the energy equation gives
	\begin{align*}
	  \bar{\phi}''+F\cdot\phi'&=0
	\end{align*}

	The change from $\eta$ to $\zeta$ coordinates is exactly the same for the mass conservation equation, which gives
	\begin{equation*}
	  \bar{S}''+\frac{\text{Sc}}{\text{Pr}}F\cdot \bar{S}'=0
	\end{equation*}

	The initial conditions can also be derived using the relations above.
	\begin{align*}
	  F(0) =& (3\text{Pr})^{3/4} f(0) = -\frac{\bar{\phi}'(0) c_p (T_0-T_\infty}{h_{il}(1-s_0/1000)}
	\end{align*}
	and since $\phi'(\eta)=(3\text{Pr})^{1/4}\bar{\phi}'(\zeta)$ and $S'(\eta)=(3\text{Pr})^{1/4}\bar{S}'(\zeta)$, the following ratio gives
	\begin{equation*}
	  \frac{S'(0)}{\phi'(0)}=\frac{\bar{S}'(0)}{\bar{\phi}'(0)} = \text{Le} \frac{c_p(T_0-T_{\infty})}{h_{il}}\cdot \frac{s_0}{(s_0-s_\infty)(1-s_0/1000)}
	\end{equation*}

	The followin initial conditions are then also tvivial
	\begin{align*}
	  F'(0) =& (3\text{Pr})^{1/2} f'(0) = 0 \\
	  \bar{\phi}(0) =& \phi (0) = 1 \qquad \bar{S}(0) = S (0) = 1 \\
	  F''(\infty) =& (3\text{Pr})^{1/4}f(\infty)=0 \\
	  \bar{\phi}(\infty) =& \phi (\infty) = 0 \qquad \bar{S}(\infty) = S (\infty) = 0 \\
	\end{align*}
	
% section Task 2 (end)


